src/go_lang/examples/logging2.v
@@ -2,9 +2,7 @@
 From Perennial.go_lang Require Import prelude.
 
 (* disk FFI *)
-From Perennial.go_lang Require Import ffi.disk.
-Existing Instances disk_op disk_model disk_ty.
-Local Coercion Var' (s: string) := Var s.
+From Perennial.go_lang Require Import ffi.disk_prelude.
 
 Definition LOGCOMMIT : expr := #0.
 
@@ -19,7 +17,7 @@ Module Log.
     "logLock" :: lockRefT;
     "memLock" :: lockRefT;
     "logSz" :: intT;
-    "memLog" :: refT (slice.T blockT);
+    "memLog" :: refT (slice.T disk.blockT);
     "memLen" :: refT intT;
     "memTxnNxt" :: refT intT;
     "logTxnNxt" :: refT intT
@@ -31,7 +29,7 @@ Module Log.
   End fields.
 End Log.
 
-Definition writeHdr: val :=
+Definition Log__writeHdr: val :=
   λ: "log" "len",
     let: "hdr" := NewSlice byteT #4096 in
     UInt64Put "hdr" "len";;
@@ -43,23 +41,23 @@ Definition Init: val :=
       "logLock" ::= Data.newLock #();
       "memLock" ::= Data.newLock #();
       "logSz" ::= "logSz";
-      "memLog" ::= ref (zero_val (slice.T blockT));
+      "memLog" ::= ref (zero_val (slice.T disk.blockT));
       "memLen" ::= ref (zero_val intT);
       "memTxnNxt" ::= ref (zero_val intT);
       "logTxnNxt" ::= ref (zero_val intT)
     ] in
-    writeHdr "log" #0;;
+    Log__writeHdr "log" #0;;
     "log".
 
-Definition readHdr: val :=
+Definition Log__readHdr: val :=
   λ: "log",
     let: "hdr" := disk.Read "LOGCOMMIT" in
     let: "disklen" := UInt64Get "hdr" in
     "disklen".
 
-Definition readBlocks: val :=
+Definition Log__readBlocks: val :=
   λ: "log" "len",
-    let: "blks" := ref (NewSlice blockT #0) in
+    let: "blks" := ref (NewSlice disk.blockT #0) in
     let: "i" := ref #0 in
     for: (!"i" < "len"); ("i" <- !"i" + #1) :=
       let: "blk" := disk.Read ("LOGSTART" + !"i") in
@@ -67,15 +65,15 @@ Definition readBlocks: val :=
       Continue;;
     !"blks".
 
-Definition Read: val :=
+Definition Log__Read: val :=
   λ: "log",
     Data.lockAcquire Writer (Log.get "logLock" "log");;
-    let: "disklen" := readHdr "log" in
-    let: "blks" := readBlocks "log" "disklen" in
+    let: "disklen" := Log__readHdr "log" in
+    let: "blks" := Log__readBlocks "log" "disklen" in
     Data.lockRelease Writer (Log.get "logLock" "log");;
     "blks".
 
-Definition memWrite: val :=
+Definition Log__memWrite: val :=
   λ: "log" "l",
     let: "n" := slice.len "l" in
     let: "i" := ref #0 in
@@ -83,7 +81,7 @@ Definition memWrite: val :=
       Log.get "memLog" "log" <- SliceAppend (!(Log.get "memLog" "log")) (SliceGet "l" !"i");;
       Continue.
 
-Definition memAppend: val :=
+Definition Log__memAppend: val :=
   λ: "log" "l",
     Data.lockAcquire Writer (Log.get "memLock" "log");;
     if: !(Log.get "memLen" "log") + slice.len "l" ≥ Log.get "logSz" "log"
@@ -99,33 +97,33 @@ Definition memAppend: val :=
       (#true, "txn").
 
 (* XXX just an atomic read? *)
-Definition readLogTxnNxt: val :=
+Definition Log__readLogTxnNxt: val :=
   λ: "log",
     Data.lockAcquire Writer (Log.get "memLock" "log");;
     let: "n" := !(Log.get "logTxnNxt" "log") in
     Data.lockRelease Writer (Log.get "memLock" "log");;
     "n".
 
-Definition diskAppendWait: val :=
+Definition Log__diskAppendWait: val :=
   λ: "log" "txn",
     Skip;;
     for: (#true); (Skip) :=
-      let: "logtxn" := readLogTxnNxt "log" in
+      let: "logtxn" := Log__readLogTxnNxt "log" in
       if: "txn" < "logtxn"
       then Break
       else Continue.
 
-Definition Append: val :=
+Definition Log__Append: val :=
   λ: "log" "l",
-    let: ("ok", "txn") := memAppend "log" "l" in
+    let: ("ok", "txn") := Log__memAppend "log" "l" in
     if: "ok"
     then
-      diskAppendWait "log" "txn";;
+      Log__diskAppendWait "log" "txn";;
       #()
     else #();;
     "ok".
 
-Definition writeBlocks: val :=
+Definition Log__writeBlocks: val :=
   λ: "log" "l" "pos",
     let: "n" := slice.len "l" in
     let: "i" := ref #0 in
@@ -134,32 +132,32 @@ Definition writeBlocks: val :=
       disk.Write ("pos" + !"i") "bk";;
       Continue.
 
-Definition diskAppend: val :=
+Definition Log__diskAppend: val :=
   λ: "log",
     Data.lockAcquire Writer (Log.get "logLock" "log");;
-    let: "disklen" := readHdr "log" in
+    let: "disklen" := Log__readHdr "log" in
     Data.lockAcquire Writer (Log.get "memLock" "log");;
     let: "memlen" := !(Log.get "memLen" "log") in
     let: "allblks" := !(Log.get "memLog" "log") in
     let: "blks" := SliceSkip "allblks" "disklen" in
     let: "memnxt" := !(Log.get "memTxnNxt" "log") in
     Data.lockRelease Writer (Log.get "memLock" "log");;
-    writeBlocks "log" "blks" "disklen";;
-    writeHdr "log" "memlen";;
+    Log__writeBlocks "log" "blks" "disklen";;
+    Log__writeHdr "log" "memlen";;
     Log.get "logTxnNxt" "log" <- "memnxt";;
     Data.lockRelease Writer (Log.get "logLock" "log").
 
-Definition Logger: val :=
+Definition Log__Logger: val :=
   λ: "log",
     Skip;;
     for: (#true); (Skip) :=
-      diskAppend "log";;
+      Log__diskAppend "log";;
       Continue.
 
 Module Txn.
   Definition S := struct.new [
     "log" :: refT Log.T;
-    "blks" :: refT (mapT blockT)
+    "blks" :: refT (mapT disk.blockT)
   ].
   Definition T: ty := struct.t S.
   Section fields.
@@ -173,11 +171,11 @@ Definition Begin: val :=
   λ: "log",
     let: "txn" := struct.mk Txn.S [
       "log" ::= "log";
-      "blks" ::= ref (zero_val (mapT blockT))
+      "blks" ::= ref (zero_val (mapT disk.blockT))
     ] in
     "txn".
 
-Definition Write: val :=
+Definition Txn__Write: val :=
   λ: "txn" "addr" "blk",
     let: (<>, "ok") := MapGet (!(Txn.get "blks" "txn")) "addr" in
     if: "ok"
@@ -194,17 +192,17 @@ Definition Write: val :=
     else #();;
     #true.
 
-Definition Read: val :=
+Definition Txn__Read: val :=
   λ: "txn" "addr",
     let: ("v", "ok") := MapGet (!(Txn.get "blks" "txn")) "addr" in
     if: "ok"
     then "v"
     else disk.Read ("addr" + "LOGEND").
 
-Definition Commit: val :=
+Definition Txn__Commit: val :=
   λ: "txn",
-    let: "blks" := ref (zero_val (slice.T blockT)) in
+    let: "blks" := ref (zero_val (slice.T disk.blockT)) in
     Data.mapIter !(Txn.get "blks" "txn") (λ: <> "v",
       "blks" <- SliceAppend !"blks" "v");;
-    let: "ok" := Append (!(Txn.get "log" "txn")) !"blks" in
+    let: "ok" := Log__Append (!(Txn.get "log" "txn")) !"blks" in
     "ok".
