src/go_lang/ffi/disk_prelude.v
@@ -1,0 +1,4 @@
+From Perennial.go_lang Require Import lang.
+From Perennial.go_lang Require ffi.disk.
+Existing Instances disk.disk_op disk.disk_ty.
+Coercion Var' (s: string) := Var s.
